\section{Euler Identity}
\label{Derivs:Euler:S}

\begin{eqnarray}
e^z&=&1+z+\frac{1}{2}z^2+\cdots + \frac{1}{n!} z^n\label{Derivs:Euler:eq:01}\\
e^{i\theta}&=&1+i\theta -\frac{1}{2}\theta^2 +\cdots\nonumber\\
&=&(1-\frac{1}{2}\theta^2 +\frac{1}{4!}\theta^4+\cdots)+i(\theta -\frac{1}{3!}\theta^3+\frac{1}{5!}\theta^5)\nonumber\\
&=&\cos(\theta)+i\sin(\theta) \label{Derivs:Euler:eq:02}\\
e^{i\pi}&=&\cos(\pi)+i\sin(\pi)\nonumber\\
&=&-1 \\
\Rightarrow 0&=&e^{i\pi}+1 \label{Derivs:Euler:eq:04}
\end{eqnarray}

Look, we can readily reference \eqref{Derivs:Euler:eq:03} in Chapter \ref{Derivs:Euler:S}.